feat: new design for automata theory, results on regular languages, and deterministic labelled transition systems (#144)
This PR merges the developments that @ctchou and I carried out in the
`automata` branch, #141, and #142, as discussed on Zulip ([#CSLib >
Question Lean structure and
extends](https://leanprover.zulipchat.com/#narrow/channel/513188-CSLib/topic/Question.20Lean.20structure.20and.20extends/with/554287177)).

The design based on `Acceptor` and structure extension works pretty
well. Some definitions could be removed because of the `Acceptor`
typeclass, and some proofs got easier thanks to the combination of
structure extension, record updates, and grind.

Co-authored with @ctchou.

---------

Co-authored-by: Ching-Tsun Chou <chingtsun.chou@gmail.com>
Co-authored-by: github-actions[bot] <41898282+github-actions[bot]@users.noreply.github.com>
Co-authored-by: Chris Henson <46805207+chenson2018@users.noreply.github.com>

Cslib/Computability/Automata/DA.lean
@@ -1,24 +1,94 @@
 /-
 Copyright (c) 2025 Fabrizio Montesi. All rights reserved.
 Released under Apache 2.0 license as described in the file LICENSE.
-Authors: Fabrizio Montesi
+Authors: Fabrizio Montesi, Ching-Tsun Chou
 -/
 
-import Cslib.Computability.Automata.NA
+import Cslib.Foundations.Semantics.LTS.FLTS
+import Cslib.Computability.Automata.Acceptor
+import Cslib.Computability.Automata.OmegaAcceptor
+import Cslib.Computability.Languages.OmegaLanguage
 
+/-! # Deterministic Automata
 
+A Deterministic Automaton (`DA`) is an automaton defined by a transition function equipped with an
+initial state.
 
-/-! # Deterministic Automaton
+Automata with different accepting conditions are then defined as extensions of `DA`.
+These include, for example, a generalised version of DFA as found in the literature (without
+finiteness assumptions), deterministic Buchi automata, and deterministic Muller automata.
 
-A Deterministic Automaton (DA) is an automaton defined by a transition function.
+## References
+
+* [J. E. Hopcroft, R. Motwani, J. D. Ullman,
+  *Introduction to Automata Theory, Languages, and Computation*][Hopcroft2006]
 -/
 
-namespace Cslib
+namespace Cslib.Automata
 
-structure DA (State : Type _) (Symbol : Type _) where
+structure DA (State Symbol : Type*) extends FLTS State Symbol where
   /-- The initial state of the automaton. -/
   start : State
-  /-- The transition function of the automaton. -/
-  tr : State → Symbol → State
 
-end Cslib
+namespace DA
+
+variable {State : Type _} {Symbol : Type _}
+
+/-- A deterministic automaton that accepts finite strings (lists of symbols). -/
+structure FinAcc (State Symbol : Type*) extends DA State Symbol where
+  /-- The accept states. -/
+  accept : Set State
+
+namespace FinAcc
+
+/-- A `DA.FinAcc` accepts a string if its multistep transition function maps the start state and
+the string to an accept state.
+
+This is the standard string recognition performed by DFAs in the literature. -/
+@[scoped grind =]
+instance : Acceptor (DA.FinAcc State Symbol) Symbol where
+  Accepts (a : DA.FinAcc State Symbol) (xs : List Symbol) := a.mtr a.start xs ∈ a.accept
+
+end FinAcc
+
+/-- Helper function for defining `run` below. -/
+@[simp, scoped grind =]
+def run' (da : DA State Symbol) (xs : ωSequence Symbol) : ℕ → State
+  | 0 => da.start
+  | n + 1 => da.tr (run' da xs n) (xs n)
+
+/-- Infinite run. -/
+@[scoped grind =]
+def run (da : DA State Symbol) (xs : ωSequence Symbol) : ωSequence State := da.run' xs
+
+open List Filter
+
+/-- Deterministic Buchi automaton. -/
+structure Buchi (State Symbol : Type*) extends DA State Symbol where
+  /-- The accept states -/
+  accept : Set State
+
+namespace Buchi
+
+@[scoped grind =]
+instance : ωAcceptor (Buchi State Symbol) Symbol where
+  Accepts (a : Buchi State Symbol) (xs : ωSequence Symbol) := ∃ᶠ k in atTop, a.run xs k ∈ a.accept
+
+end Buchi
+
+/-- Deterministic Muller automaton. -/
+structure Muller (State Symbol : Type*) extends DA State Symbol where
+  /-- The accepting set of sets of states. -/
+  accept : Set (Set State)
+
+namespace Muller
+
+@[scoped grind =]
+instance : ωAcceptor (Muller State Symbol) Symbol where
+  Accepts (a : Muller State Symbol) (xs : ωSequence Symbol) := (a.run xs).infOcc ∈ a.accept
+
+end Muller
+
+end DA
+
+end Cslib.Automata
