Cslib/Computability/Automata/NA.lean
@@ -1,24 +1,94 @@
 /-
 Copyright (c) 2025 Fabrizio Montesi. All rights reserved.
 Released under Apache 2.0 license as described in the file LICENSE.
-Authors: Fabrizio Montesi
+Authors: Fabrizio Montesi, Ching-Tsun Chou
 -/
 
+import Cslib.Computability.Languages.OmegaLanguage
 import Cslib.Foundations.Semantics.LTS.Basic
+import Cslib.Foundations.Semantics.LTS.FLTS
+import Cslib.Computability.Automata.Acceptor
+import Cslib.Computability.Automata.OmegaAcceptor
 
 /-! # Nondeterministic Automaton
 
-A Nondeterministic Automaton (NA) is an automaton with a set of initial states.
+A Nondeterministic Automaton (NA) is a transition relation equipped with a set of initial states.
+
+Automata with different accepting conditions are then defined as extensions of `NA`.
+These include, for example, a generalised version of NFA as found in the literature (without
+finiteness assumptions), nondeterministic Buchi automata, and nondeterministic Muller automata.
 
 This definition extends `LTS` and thus stores the transition system as a relation `Tr` of the form
 `State → Symbol → State → Prop`. Note that you can also instantiate `Tr` by passing an argument of
 type `State → Symbol → Set State`; it gets automatically expanded to the former shape.
+
+## References
+
+* [J. E. Hopcroft, R. Motwani, J. D. Ullman,
+  *Introduction to Automata Theory, Languages, and Computation*][Hopcroft2006]
 -/
 
-namespace Cslib
+open Filter
 
-structure NA (State : Type _) (Symbol : Type _) extends LTS State Symbol where
+namespace Cslib.Automata
+
+structure NA (State Symbol : Type*) extends LTS State Symbol where
   /-- The set of initial states of the automaton. -/
   start : Set State
 
-end Cslib
+namespace NA
+
+variable {State : Type _} {Symbol : Type _}
+
+/-- A nondeterministic automaton that accepts finite strings (lists of symbols). -/
+structure FinAcc (State Symbol : Type*) extends NA State Symbol where
+  /-- The accept states. -/
+  accept : Set State
+
+namespace FinAcc
+
+/-- An `NA.FinAcc` accepts a string if there is a multistep transition from a start state to an
+accept state.
+
+This is the standard string recognition performed by NFAs in the literature. -/
+@[scoped grind =]
+instance : Acceptor (FinAcc State Symbol) Symbol where
+  Accepts (a : FinAcc State Symbol) (xs : List Symbol) :=
+    ∃ s ∈ a.start, ∃ s' ∈ a.accept, a.MTr s xs s'
+
+end FinAcc
+
+/-- Infinite run. -/
+@[scoped grind =]
+def Run (na : NA State Symbol) (xs : ωSequence Symbol) (ss : ωSequence State) :=
+  ss 0 ∈ na.start ∧ ∀ n, na.Tr (ss n) (xs n) (ss (n + 1))
+
+/-- Nondeterministic Buchi automaton. -/
+structure Buchi (State Symbol : Type*) extends NA State Symbol where
+  accept : Set State
+
+namespace Buchi
+
+@[scoped grind =]
+instance : ωAcceptor (Buchi State Symbol) Symbol where
+  Accepts (a : Buchi State Symbol) (xs : ωSequence Symbol) :=
+    ∃ ss, ∃ᶠ k in atTop, a.Run xs ss ∧ ss k ∈ a.accept
+
+end Buchi
+
+/-- Nondeterministic Muller automaton. -/
+structure Muller (State Symbol : Type*) extends NA State Symbol where
+  accept : Set (Set State)
+
+namespace Muller
+
+@[scoped grind =]
+instance : ωAcceptor (Muller State Symbol) Symbol where
+  Accepts (a : Muller State Symbol) (xs : ωSequence Symbol) :=
+    ∃ ss, a.Run xs ss ∧ ss.infOcc ∈ a.accept
+
+end Muller
+
+end NA
+
+end Cslib.Automata
