Cslib/Computability/Automata/DAToNA.lean
@@ -1,0 +1,53 @@
+/-
+Copyright (c) 2025 Fabrizio Montesi. All rights reserved.
+Released under Apache 2.0 license as described in the file LICENSE.
+Authors: Fabrizio Montesi
+-/
+
+import Cslib.Computability.Automata.DA
+import Cslib.Computability.Automata.NA
+import Cslib.Foundations.Semantics.LTS.FLTSToLTS
+
+/-! # Translation of Deterministic Automata into Nonodeterministic Automata.
+
+This is the general version of the standard translation of DFAs into NFAs. -/
+
+namespace Cslib.Automata.DA
+
+variable {State : Type _} {Symbol : Type _}
+
+section NA
+
+/-- `DA` is a special case of `NA`. -/
+@[scoped grind =]
+def toNA (a : DA State Symbol) : NA State Symbol :=
+  { a.toLTS with start := {a.start} }
+
+instance : Coe (DA State Symbol) (NA State Symbol) where
+  coe := toNA
+
+namespace FinAcc
+
+/-- `DA.FinAcc` is a special case of `NA.FinAcc`. -/
+@[scoped grind =]
+def toNAFinAcc (a : DA.FinAcc State Symbol) : NA.FinAcc State Symbol :=
+  { a.toNA with accept := a.accept }
+
+open Acceptor in
+open scoped FLTS NA.FinAcc in
+/-- The `NA` constructed from a `DA` has the same language. -/
+@[scoped grind _=_]
+theorem toNAFinAcc_language_eq {a : DA.FinAcc State Symbol} :
+    language a.toNAFinAcc = language a := by
+  ext xs
+  constructor
+  · grind
+  · intro _
+    use a.start
+    grind
+
+end FinAcc
+
+end NA
+
+end Cslib.Automata.DA
