Cslib/Computability/Automata/EpsilonNA.lean
@@ -1,0 +1,51 @@
+/-
+Copyright (c) 2025 Fabrizio Montesi. All rights reserved.
+Released under Apache 2.0 license as described in the file LICENSE.
+Authors: Fabrizio Montesi, Ching-Tsun Chou
+-/
+
+import Cslib.Computability.Automata.NA
+import Cslib.Computability.Automata.Acceptor
+
+/-! # Nondeterministic automata with ε-transitions. -/
+
+namespace Cslib.Automata
+
+/-- A nondeterministic finite automaton with ε-transitions (`εNA`) is an `NA` with an `Option`
+symbol type. The special symbol ε is represented by the `Option.none` case.
+
+Internally, ε (`Option.none`) is treated as the `τ` label of the underlying transition system,
+allowing for reusing the definitions and results on saturated transitions of `LTS` to deal with
+ε-closure. -/
+structure εNA (State Symbol : Type*) extends NA State (Option Symbol)
+
+variable {State Symbol : Type*}
+
+@[local grind =]
+private instance : HasTau (Option α) := ⟨.none⟩
+
+/-- The `ε`-closure of a set of states `S` is the set of states reachable by any state in `S`
+by performing only `ε`-transitions. We use `LTS.τClosure` since `ε` (`Option.none`) is an instance
+of `HasTau.τ`. -/
+abbrev εNA.εClosure (a : εNA State Symbol) (S : Set State) := a.τClosure S
+
+namespace εNA
+
+structure FinAcc (State Symbol : Type*) extends εNA State Symbol where
+  accept : Set State
+
+namespace FinAcc
+
+/-- An `εNA.FinAcc` accepts a string if there is a saturated multistep accepting derivative with
+that trace from the start state. -/
+@[scoped grind =]
+instance : Acceptor (FinAcc State Symbol) Symbol where
+  Accepts (a : FinAcc State Symbol) (xs : List Symbol) :=
+    ∃ s ∈ a.εClosure a.start, ∃ s' ∈ a.accept,
+    a.saturate.MTr s (xs.map (some ·)) s'
+
+end FinAcc
+
+end εNA
+
+end Cslib.Automata
