Cslib/Computability/Automata/NAToDA.lean
@@ -1,0 +1,52 @@
+/-
+Copyright (c) 2025 Fabrizio Montesi. All rights reserved.
+Released under Apache 2.0 license as described in the file LICENSE.
+Authors: Fabrizio Montesi
+-/
+
+import Cslib.Computability.Automata.DA
+import Cslib.Computability.Automata.NA
+import Cslib.Foundations.Semantics.LTS.LTSToFLTS
+
+/-! # Translation of Nondeterministic Automata for finite strings into Deterministic Automata
+
+This file implements the standard subset construction.
+-/
+
+namespace Cslib.Automata.NA
+
+variable {State : Type _} {Symbol : Type _}
+
+section SubsetConstruction
+
+/-- Converts an `NA` into a `DA` using the subset construction. -/
+@[scoped grind =]
+def toDA (a : NA State Symbol) : DA (Set State) Symbol :=
+  { a.toFLTS with start := a.start }
+
+namespace FinAcc
+
+/-- Converts an `NA.FinAcc` into a `DA.FinAcc` using the subset construction. -/
+@[scoped grind =]
+def toDAFinAcc (a : NA.FinAcc State Symbol) : DA.FinAcc (Set State) Symbol :=
+  { a.toDA with accept := { S | ∃ s ∈ S, s ∈ a.accept } }
+
+open Acceptor in
+open scoped DA.FinAcc LTS in
+/-- The `DA` constructed from an `NA` has the same language. -/
+@[scoped grind _=_]
+theorem toDAFinAcc_language_eq {na : NA.FinAcc State Symbol} :
+  language na.toDAFinAcc = language na := by
+  ext xs
+  #adaptation_note
+  /--
+  Moving from `nightly-2025-09-15` to `nightly-2025-10-19` required
+  increasing the number of allowed splits.
+  -/
+  grind (splits := 11)
+
+end FinAcc
+
+end SubsetConstruction
+
+end Cslib.Automata.NA
