Cslib/Computability/Automata/OmegaAcceptor.lean
@@ -1,0 +1,32 @@
+/-
+Copyright (c) 2025 Fabrizio Montesi. All rights reserved.
+Released under Apache 2.0 license as described in the file LICENSE.
+Authors: Fabrizio Montesi
+-/
+
+import Cslib.Computability.Languages.OmegaLanguage
+
+namespace Cslib.Automata
+
+/-- An `ωAcceptor` is a machine that recognises infinite sequences of symbols. -/
+class ωAcceptor (A : Type _) (Symbol : outParam (Type _)) where
+  /-- Predicate that establishes whether a string `xs` is accepted. -/
+  Accepts (a : A) (xs : ωSequence Symbol) : Prop
+
+namespace ωAcceptor
+
+variable {Symbol : Type _}
+
+/-- The language of an `ωAcceptor` is the set of sequences it `Accepts`. -/
+@[scoped grind .]
+def language [ωAcceptor A Symbol] (a : A) : ωLanguage Symbol :=
+  { xs | Accepts a xs }
+
+/-- A string is in the language of an acceptor iff the acceptor accepts it. -/
+@[scoped grind =]
+theorem mem_language [ωAcceptor A Symbol] (a : A) (xs : ωSequence Symbol) :
+  xs ∈ language a ↔ Accepts a xs := Iff.rfl
+
+end ωAcceptor
+
+end Cslib.Automata
