Cslib/Computability/Languages/OmegaRegularLanguage.lean
@@ -1,0 +1,39 @@
+/-
+Copyright (c) 2025 Ching-Tsun Chou. All rights reserved.
+Released under Apache 2.0 license as described in the file LICENSE.
+Authors: Ching-Tsun Chou
+-/
+
+import Cslib.Computability.Automata.DA
+import Cslib.Computability.Automata.NA
+import Mathlib.Tactic
+
+/-!
+# ω-Regular languages
+
+This file defines ω-regular languages and proves some properties of them.
+-/
+
+open Set Function
+open scoped Computability
+open Cslib.Automata
+
+namespace Cslib.ωLanguage
+
+variable {Symbol : Type*}
+
+/-- An ω-regular language is one that is accepted by a finite-state Buchi automaton. -/
+def IsRegular (p : ωLanguage Symbol) :=
+  ∃ State : Type, ∃ _ : Finite State, ∃ na : NA.Buchi State Symbol, ωAcceptor.language na = p
+
+/-- There is an ω-regular language which is not accepted by any deterministic Buchi automaton. -/
+proof_wanted IsRegular.not_det_buchi :
+  ∃ p : ωLanguage Symbol, p.IsRegular ∧
+    ¬ ∃ State : Type, ∃ _ : Finite State, ∃ da : DA.Buchi State Symbol, ωAcceptor.language da = p
+
+/-- McNaughton's Theorem. -/
+proof_wanted IsRegular.iff_muller_lang {p : ωLanguage Symbol} :
+    p.IsRegular ↔
+    ∃ State : Type, ∃ _ : Finite State, ∃ da : DA.Muller State Symbol, ωAcceptor.language da = p
+
+end Cslib.ωLanguage
