Cslib/Foundations/Data/OmegaSequence/Defs.lean
@@ -7,6 +7,7 @@ import Cslib.Init
 import Mathlib.Data.Nat.Notation
 import Mathlib.Data.FunLike.Basic
 import Mathlib.Logic.Function.Iterate
+import Mathlib.Order.Filter.AtTopBot.Defs
 
 /-!
 # Definition of `ωSequence` and functions on infinite sequences
@@ -22,6 +23,8 @@ Most code below is adapted from Mathlib.Data.Stream.Defs.
 -/
 
 namespace Cslib
+
+open Filter
 
 universe u v w
 variable {α : Type u} {β : Type v} {δ : Type w}
@@ -84,6 +87,10 @@ def zip (f : α → β → δ) (s₁ : ωSequence α) (s₂ : ωSequence β) : �
 
 /-- Iterates of a function as an ω-sequence. -/
 def iterate (f : α → α) (a : α) : ωSequence α := fun n => f^[n] a
+
+/-- The set of elements that appear infinitely often in an ω-sequence. -/
+def infOcc (xs : ωSequence α) : Set α :=
+  { x | ∃ᶠ k in atTop, xs k = x }
 
 end ωSequence
 
