Cslib/Foundations/Semantics/LTS/FLTS.lean
@@ -1,0 +1,49 @@
+/-
+Copyright (c) 2025 Fabrizio Montesi. All rights reserved.
+Released under Apache 2.0 license as described in the file LICENSE.
+Authors: Fabrizio Montesi
+-/
+
+import Cslib.Init
+
+/-! # Functional Labelled Transition System (FLTS)
+
+A Functional Labelled Transition System is a special case of an `LTS` where transitions are
+determined by a function.
+
+This is a generalisation of deterministic finite-state machines.
+
+## References
+
+* [J. E. Hopcroft, R. Motwani, J. D. Ullman,
+  *Introduction to Automata Theory, Languages, and Computation*][Hopcroft2006]
+-/
+
+namespace Cslib
+
+/--
+A Functional Labelled Transition System (`FLTS`) for a type of states (`State`) and a type of
+transition labels (`Label`) consists of a labelled transition function (`tr`).
+-/
+structure FLTS (State : Type _) (Label : Type _) where
+  /-- The transition function. -/
+  tr : State → Label → State
+
+namespace FLTS
+
+variable {State : Type _} {Label : Type _}
+
+/-- Extended transition function.
+
+Implementation note: compared to [Hopcroft2006], the definition consumes the input list of symbols
+from the left (instead of the right), in order to match the way lists are constructed.
+-/
+@[scoped grind =]
+def mtr (flts : FLTS State Label) (s : State) (μs : List Label) := μs.foldl flts.tr s
+
+@[scoped grind =]
+theorem mtr_nil_eq {flts : FLTS State Label} {s : State} : flts.mtr s [] = s := rfl
+
+end FLTS
+
+end Cslib
