Cslib/Foundations/Semantics/LTS/LTSToFLTS.lean
@@ -1,0 +1,46 @@
+/-
+Copyright (c) 2025 Fabrizio Montesi. All rights reserved.
+Released under Apache 2.0 license as described in the file LICENSE.
+Authors: Fabrizio Montesi
+-/
+
+import Cslib.Foundations.Semantics.LTS.FLTS
+import Cslib.Foundations.Semantics.LTS.Basic
+
+variable {State : Type _} {Label : Type _}
+
+namespace Cslib.LTS
+
+/-- Converts an `LTS` into an `FLTS` using the subset construction. -/
+@[scoped grind =]
+def toFLTS (lts : LTS State Label) : FLTS (Set State) Label where
+  tr := lts.setImage
+
+/-- Characterisation of transitions in `LTS.toFLTS` wrt transitions in the original `LTS`. -/
+@[scoped grind =]
+theorem toFLTS_mem_tr {lts : LTS State Label} {S : Set State} {s' : State} {μ : Label} :
+  s' ∈ lts.toFLTS.tr S μ ↔ ∃ s ∈ S, lts.Tr s μ s' := by
+  simp only [LTS.toFLTS, LTS.setImage, Set.mem_iUnion, exists_prop]
+  grind
+
+/-- Characterisation of multistep transitions in `LTS.toFLTS` wrt multistep transitions in the
+original `LTS`. -/
+@[scoped grind =]
+theorem toFLTS_mem_mtr {lts : LTS State Label} {S : Set State} {s' : State} {μs : List Label} :
+  s' ∈ lts.toFLTS.mtr S μs ↔ ∃ s ∈ S, lts.MTr s μs s' := by
+  simp only [LTS.toFLTS, FLTS.mtr]
+  /- TODO: Grind does not catch a useful rewrite in the subset construction for automata
+
+    A very similar issue seems to occur in the proof of `LTS.toFLTS_language_eq`.
+
+    labels: grind, lts, automata
+  -/
+  rw [← LTS.setImageMultistep_foldl_setImage]
+  grind
+
+/-- Characterisation of multistep transitions in `LTS.toFLTS` as image transitions in `LTS`. -/
+@[scoped grind =]
+theorem toFLTS_mtr_setImageMultistep {lts : LTS State Label} :
+  lts.toFLTS.mtr = lts.setImageMultistep := by grind
+
+end Cslib.LTS
